Start some lemmas

coq/common/defs/obj.v
@@ -2,7 +2,7 @@
 (* Objects *)
 (* =================================================== *)
 
-Unset Automatic Proposition Inductives.
+(* Unset Automatic Proposition Inductives. *)
 
-Inductive obj : Type := .
-(* Variable obj : Type. *)
+(* Inductive obj : Type := . *)
+Parameter obj : Type.
