coq/common/defs/obj2.v
@@ -22,26 +22,18 @@ Inductive obj_eq : obj -> obj -> Type :=
 (* IsVar [Ψ ⊢ X]: X is a parameter variable under the LF context Ψ *)
 
 Inductive IsVar : ctx -> obj -> Prop :=
-| IsVar_intro : forall (Ψ : ctx) (p : obj), IsVar (extend p Ψ) p.
+| IsVar_intro : forall (psi : ctx) (p : obj), IsVar (extend p psi) p.
 
 (* Definition for 'pruning' LF context to remove dependencies *)
 
 Inductive PruneObj : ctx -> (obj -> obj) -> Prop :=
-| Prune_Obj : forall (Ψ : ctx) (M : obj -> obj),
-    PruneObj Ψ M.
+| Prune_Obj : forall (psi : ctx) (M : obj -> obj),
+    PruneObj psi M.
 
 (* CompareObjs: compares two objects to indicate if they are equal or unequal *)
+(* Inductive type to encode the property that for any objects M and N, either M = N or M ≠ N *)
+(* (see, e.g., the lemma comp_obj in common/lemmas/obj2.bel) *)
 
-Inductive CompareObjs (Ψ : ctx) (M N : obj) : Prop :=
-| Ct_Eq : M = N -> CompareObjs Ψ M N
-| Ct_Neq : M <> N -> CompareObjs Ψ M N.
-
-(* 
-Record ctx := {
-element : obj
-}. *)
-
-(* Inductive CompareObjs : ctx -> obj -> obj -> Type :=
-| Ct_Eq : forall (Ψ : ctx) (M : obj), CompareObjs Ψ M M
-| Ct_Neq : forall (Ψ : ctx) (M N : obj),
-    (obj_eq M N -> False) -> CompareObjs Ψ M N. *)
+Inductive CompareObjs (psi : ctx) (M N : obj) : Prop :=
+| Ct_Eq : M = N -> CompareObjs psi M N
+| Ct_Neq : M <> N -> CompareObjs psi M N.
