coq/common/defs/ctx.v
@@ -17,7 +17,6 @@ Inductive lctx : nat -> Type :=
 
 (* Typing context equality *)
 
-(* curly braces *)
 (* https://coq.inria.fr/doc/v8.12/refman/language/extensions/implicit-arguments.html *)
 
 Inductive cx_eq {N : nat} : lctx N -> lctx N -> Type :=
@@ -38,8 +37,98 @@ Inductive merge : forall {N : nat}, lctx N -> lctx N -> lctx N -> Type :=
     -> mult_op alpha1 alpha2 alpha
     -> merge (cons N delta1 X A alpha1) (cons N delta2 X A alpha2) (cons N delta X A alpha).
 
+(* Δ[x :α A ↦ₙ y :β B] = Δ' *)
+(* i.e., x appears in Δ at position n with type A and multiplicity α, and *)
+(* Δ' is the result of changing that entry to y :β B *)
+
+Inductive upd : forall {N : nat}, lctx N -> nat -> obj -> obj -> tp -> tp -> mult -> mult -> lctx N -> Type :=
+| upd_t : forall {N : nat} (delta : lctx N) (X X' : obj) (A A' : tp) (alpha alpha' : mult),
+    upd (cons N delta X A alpha) (S N) X X' A A' alpha alpha' (cons N delta X' A' alpha')
+| upd_n : forall {N : nat} (delta delta' : lctx N) (n : nat) (X X' Y : obj) (A A' B : tp) (alpha alpha' beta : mult),
+    upd delta n X X' A A' alpha alpha' delta' ->
+    upd (cons N delta Y B beta) n X X' A A' alpha alpha' (cons N delta' Y B beta).
+
+(* Only unrestricted assumptions appear in Δ, *)
+(* parametric to the predicate "unr α"; in the case of linear type systems, *)
+(* "unr α" holds when α = 𝟘 (unavailable). *)
+
+Inductive exh : forall {N : nat}, lctx N -> Prop :=
+| exh_n : exh nil
+| exh_c : forall {N : nat} (delta : lctx N) (x : obj) (A : tp) (alpha : mult),
+    exh delta -> unr alpha -> exh (cons N delta x A alpha).
+
+(* Δ ≈ Δ', Δ = Δ' up to varying multiplicities *)
+(* (corresponds to 0Δ = 0Δ' for linear systems) *)
+
+Inductive same_elts : forall {N : nat}, lctx N -> lctx N -> Type :=
+| se_n : same_elts nil nil
+| se_c : forall {N : nat} (delta delta' : lctx N) (X : obj) (A : tp) (alpha alpha' : mult),
+    same_elts delta delta' -> same_elts (cons N delta X A alpha) (cons N delta' X A alpha').
+
 (* --------------------------------------------------- *)
-(* Context pruning *)
+(* Shorthand for other properties *)
 (* --------------------------------------------------- *)
 
+(* Δ[(n, x) ↔ (m, y)] = Δ', i.e., permute two distinct elements of a typing context *)
 
+(* Exchanging two distinct elements in a typing context *)
+Inductive exch : forall {N : nat}, lctx N -> nat -> obj -> nat -> obj -> lctx N -> Type :=
+| exch_u : forall {N : nat} (delta delta' delta'' : lctx N) (n m : nat) (x y : obj) (a b : tp) (alpha beta : mult),
+    n <> m ->                        (* Ensure n and m are distinct *)
+    upd delta n x y a b alpha beta delta'' ->    (* Update at position n *)
+    upd delta'' m y x b a beta alpha delta' ->   (* Update at position m *)
+    exch delta n x m y delta'.                   (* Resulting context after exchange *)
+
+
+(* Look up name, type, and multiplicity *)
+
+Inductive lookup : obj -> tp -> mult -> forall {N : nat}, lctx N -> Prop :=
+| look : forall {N : nat} (delta delta' : lctx N) (X : obj) (A : tp) (alpha : mult) (n : nat),
+    upd delta n X X A A alpha alpha delta' -> lookup X A alpha delta.
+
+
+(* Look up name *)
+
+Inductive lookup_n : obj -> forall {N : nat}, lctx N -> Prop :=
+| lookn : forall {N : nat} (delta delta' : lctx N) (X : obj) (A : tp) (alpha : mult) (n : nat),
+    upd delta n X X A A alpha alpha delta' -> lookup_n X delta.
+
+(* Look up index and name *)
+
+Inductive lookup_in : nat -> obj -> forall {N : nat}, lctx N -> Prop :=
+| lookin : forall {N : nat} (delta delta' : lctx N) (n : nat) (X Y : obj) (A B : tp) (alpha beta : mult),
+    upd delta n X Y A B alpha beta delta' -> lookup_in n X delta.
+
+(* Look up index, name, and type *)
+
+Inductive lookup_int : nat -> obj -> tp -> forall {N : nat}, lctx N -> Prop :=
+| lookint : forall {N : nat} (delta delta' : lctx N) (n : nat) (X Y : obj) (A B : tp) (alpha beta : mult),
+    upd delta n X Y A B alpha beta delta' -> lookup_int n X A delta.
+
+(* Look up index, name, type, and multiplicity *)
+
+Inductive lookup_intm : nat -> obj -> tp -> mult -> forall {N : nat}, lctx N -> Prop :=
+| lookintm : forall {N : nat} (delta delta' : lctx N) (n : nat) (X Y : obj) (A B : tp) (alpha beta : mult),
+    upd delta n X Y A B alpha beta delta' -> lookup_intm n X A alpha delta.
+
+(* --------------------------------------------------- *)
+(* Well-formedness conditions *)
+(* --------------------------------------------------- *)
+
+(* Context contains no duplicate names and only elements of the LF context *)
+
+Inductive Wf : forall {N : nat}, lctx N -> Prop :=
+| Wf_nil : Wf nil
+| Wf_cons : forall {N : nat} (delta : lctx N) (x : obj) (A : tp) (alpha : mult),
+    Wf delta ->
+    (forall n : nat, ~ lookup_n x delta) ->  (* Ensure x does not already exist in delta *)
+    Wf (cons N delta x A alpha).
+
+(* TODO Ask if missing anuthing *)
+(* Context contains only variables from the LF context *)
+
+Inductive VarCtx : forall {N : nat}, lctx N -> Prop :=
+| VCtx_nil : VarCtx nil
+| VCtx_cons : forall {N : nat} (delta : lctx N) (p : obj) (A : tp) (alpha : mult),
+    VarCtx delta ->
+    VarCtx (cons N delta p A alpha).
