coq/common/lemmas/merge/cancl.v
@@ -1,0 +1,17 @@
+(* =================================================== *)
+(* Algebraic properties that depend on *)
+(* resource algebra operation being cancellative *)
+(* =================================================== *)
+
+Require Import common.ctx.
+Require Import common.obj2.
+
+(* Cancellativity: If Δ₁ ⋈ Δ₂ = Δ₁ ⋈ Δ₂', then Δ₂ = Δ₂' *)
+Lemma merge_cancl_lemma :
+  forall (psi : ctx) (N : nat) (delta delta1 delta2 delta2' : lctx N),
+    merge delta1 delta2 delta ->
+    merge delta1 delta2' delta ->
+    cx_eq delta2 delta2'.
+Proof.
+Admitted.
+
