coq/common/lemmas/merge/main.v
@@ -1,0 +1,61 @@
+(* =================================================== *)
+(* Properties of context merge *)
+(* =================================================== *)
+
+Require Import common.obj2.
+Require Import common.ctx.
+Require Import common.tp.
+Require Import common.obj.
+Require Import common.mult.lin_aff.
+
+(* Basic properties of judgment *)
+
+(* "Prune" LF context to remove dependencies: *)
+(* (1) Obtain from [Ψ,x:obj ⊢ merge Δ₁ Δ₂ Δ[..]] that neither Δ₁ nor Δ₂ depend on x *)
+(* (2) Obtain from [Ψ,x:obj ⊢ merge Δ₁[..] Δ₂ Δ] that neither Δ₂ nor Δ depend on x *)
+
+Inductive PruneMerge : ctx -> forall {N : nat}, lctx N -> lctx N -> lctx N -> Prop :=
+| Prune_Merge_n : forall Psi, PruneMerge Psi nil nil nil
+| Prune_Merge_c : forall Psi {N : nat} (delta1 delta2 delta : lctx N) (X : obj) (A : tp) 
+                    (alpha1 alpha2 alpha : mult),
+    PruneMerge Psi delta1 delta2 delta ->
+    mult_op alpha1 alpha2 alpha ->
+    PruneMerge Psi (cons N delta1 X A alpha1) (cons N delta2 X A alpha2) (cons N delta X A alpha).
+
+(* PruneMerge lemma, structured with induction over merge *)
+Lemma prune_merge :
+  forall (Psi : ctx) {N : nat} (Delta : lctx N) (Delta1 Delta2 : lctx N),
+    merge Delta1 Delta2 Delta -> 
+    PruneMerge Psi Delta1 Delta2 Delta.
+Proof.
+  intros Psi N Delta Delta1 Delta2 Hmerge.
+  induction Hmerge.
+  - (* Base case: mg_n *)
+    apply Prune_Merge_n.
+  - (* Recursive case: mg_c *)
+    apply Prune_Merge_c.
+    + apply IHHmerge. (* Apply the induction hypothesis *)
+    + assumption. (* Apply mult_op condition directly *)
+Qed.
+
+Lemma prune_merge_l :
+  forall (Psi : ctx) {N : nat} (Delta : lctx N) (Delta1 Delta2 : lctx N),
+    merge Delta1 Delta2 Delta ->
+    PruneMerge Psi Delta1 Delta2 Delta.
+Proof.
+  intros Psi N Delta Delta1 Delta2 Hmerge.
+  induction Hmerge.
+  - (* Base case: mg_n *)
+    apply Prune_Merge_n.
+  - (* Recursive case: mg_c *)
+    apply Prune_Merge_c.
+    + apply IHHmerge. (* Use the induction hypothesis for Delta1 and Delta2 *)
+    + assumption. (* Apply the mult_op property directly *)
+Qed.
+
+(* --------------------------------------------------- *)
+(* Algebraic properties *)
+(* --------------------------------------------------- *)
+
+(* Functionality: If Δ₁ ⋈ Δ₂ = Δ and Δ₁ ⋈ Δ₂ = Δ', then Δ = Δ' *)
+
