coq/common/lemmas/mult_lemma/lin_aff.v
@@ -1,0 +1,23 @@
+(* =================================================== *)
+(* Algebraic properties of multiplicities *)
+(* (linear / affine systems) *)
+(* =================================================== *)
+
+(* Remark: • is not total since 𝟙 • 𝟙 is undefined *)
+
+Require Import common.mult.lin_aff.
+
+(* Functionality: If α₁ ∙ α₂ = α and α₁ ∙ α₂ = α', then α = α' *)
+
+Lemma mult_func :
+  forall (alpha1 alpha2 alpha alpha' : mult),
+    mult_op alpha1 alpha2 alpha ->
+    mult_op alpha1 alpha2 alpha' ->
+    mult_eq alpha alpha'.
+Proof.
+  intros alpha1 alpha2 alpha alpha' Hmult1 Hmult2.
+  (* Case analysis on Hmult1 to match possible forms of mult_op *)
+  destruct Hmult1;
+  inversion Hmult2; subst;
+  apply mult_refl.
+Qed.
