coq/common/lemmas/obj_lemma.v
@@ -1,0 +1,70 @@
+(* =================================================== *)
+(* General properties of objects *)
+(* =================================================== *)
+
+Require Import common.obj.
+Require Import common.obj2.
+
+(* TODO TO BE VERIFIED *)
+
+(* Weaken object inequality judgment *)
+Lemma neq_weak_v :
+  forall (Psi : ctx) (M N : obj),
+    (obj_eq M N -> False) -> (forall x : obj, obj_eq M N -> False).
+Proof.
+  intros Psi M N neq_proof x eq_proof.
+  (* Since `obj_eq M N -> False`, any instance of `obj_eq M N` leads to contradiction *)
+  apply neq_proof in eq_proof. (* Apply the `neq_proof` to derive contradiction *)
+  contradiction.
+Qed.
+
+(* Object inequality is commutative *)
+Lemma neq_comm_v :
+  forall (Psi : ctx) (M N : obj),
+    (obj_eq M N -> False) -> (obj_eq N M -> False).
+Proof.
+  intros Psi M N neq_proof eq_proof.
+  (* Use symmetry if `obj_eq` is symmetric *)
+  assert (sym_eq : obj_eq M N).
+  { inversion eq_proof; subst. apply obj_refl. } (* Use `obj_refl` to show `obj_eq M N` *)
+  apply neq_proof in sym_eq. (* Now we can apply `neq_proof` to get a contradiction *)
+  contradiction.
+Qed.
+
+(*
+(* Symmetry of object equality *)
+Lemma obj_eq_sym : forall (M N : obj), obj_eq M N -> obj_eq N M.
+Proof.
+  intros M N H.
+  destruct H.
+  apply obj_refl.
+Qed.
+
+(* =================================================== *)
+(* Weaken object inequality judgment *)
+(* =================================================== *)
+
+Lemma neq_weak_v :
+  forall (Psi : ctx) (M N : obj),
+    (obj_eq M N -> False) -> (forall x : obj, obj_eq M N -> False).
+Proof.
+  intros Psi M N neq_proof x eq_proof.
+  apply neq_proof.
+  exact eq_proof.
+Qed.
+
+(* =================================================== *)
+(* Object inequality is commutative *)
+(* =================================================== *)
+
+Lemma neq_comm_v :
+  forall (Psi : ctx) (M N : obj),
+    (obj_eq M N -> False) -> (obj_eq N M -> False).
+Proof.
+  intros Psi M N neq_proof eq_proof.
+  apply neq_proof.
+  apply obj_eq_sym.
+  exact eq_proof.
+Qed. 
+
+*)
